refactor: remove rfsfun and refactor proofs
To ensure lab, fpred and frf are defined over the same domain I merged
those three functions into one function returning a triple.

eventstructure.v
@@ -1,42 +1,38 @@
-From Coq Require Import Relations.
+From Coq Require Import Relations Relation_Operators.
 From mathcomp Require Import ssreflect ssrfun ssrbool ssrnat seq path.
 From mathcomp Require Import eqtype choice order finmap.
-From event_struct Require Import utilities relations rfsfun wftype ident.
+From event_struct Require Import utilities relations wftype ident.
 
 (******************************************************************************)
 (* This file contains the definitions of:                                     *)
-(*     fin_exec_event_structure d E == definition of finite execution event   *)
-(*                              structure where E : identType d               *)
-(*           label R W == label that can be: Read x a, Write x a, ThreadEnd   *)
-(*                      or ThreadStart                                        *)
-(*           w << r == r can read from w                                      *)
-(* --> it_contains:                                                           *)
-(*          1) dom : seq E == all elements of our event structure. It should  *)
-(*                   by sorted because we want to create a fresh element,     *)
-(*                   that is not in dom just by taking fresh of it's biggest  *)
-(*                   element                                                  *)
-(*          2) lab : rfsfun (fun=> ThreadEnd) dom (fun _ _ => true)           *)
-(*                    == labeling finite function on dom, that returns        *)
-(*                   ThreadEnd if out of domain                               *)
-(*          3) ffpred : rfsfun id dom (>=%O) == finite function that returns  *)
-(*                  predsessor of arbitrary element x if he has one, or x     *)
-(*                  otherwise                                                 *)
-(*          4) ffrf   :                                                       *)
-(*             rfsufn id dom                                                  *)
-(*             [rel r w : E | (w <= r) && ((w == r) (+) ((lab w) << (lab r)))]*)
-(*             == finite function that by x returns element form that x reads *)
+(* Event labels:                                                              *)
+(*   label R W == an event label telling its type: read, write, the start of  *)
+(*                of a thread or the end of a thread                          *)
+(*      w << r == an event labelled `r` reads from an event labelled `w`      *)
+(*                                                                            *)
+(* Finite execution event structures:                                         *)
+(*   fin_exec_event_structure d E == definition of a finite execution event   *)
+(*                                   structure where E : identType d          *)
+(*     dom == the sorted sequences of events of the event structure. It is    *)
+(*            sorted in the descending order to make issuing fresh events     *)
+(*            a constant time operation.                                      *)
+(*   lab e == the label of the event e; lab is a finitely supported function  *)
+(*            defined on dom; returns ThreadEnd for the events outside of     *)
+(*            dom.                                                            *)
+(* fpred e == the predecessor of the event e, fpred is a finitely supported   *)
+(*            function that returns e if e is outside of dom.                 *)
+(*   frf e == finite function that by x returns element form that x reads     *)
 (*              if lab x = Read and x otherwise                               *)
-(* Then we are trying to derive some theory of finite event structure:        *)
-(*               ica x y iff x = ffred y or x = ffrf y                        *)
-(*               ca == casuality relation (just reflexive-transitive closure  *)
-(*                  of ica                                                    *)
-(*               cf == conflict relation (e1 # e2 -- notation for cf e1 e2)   *)
-(* If we ask that reads are not in conflict with the writes where they read   *)
-(* from, we can prove irreflexivity of our conflict relation.                 *)
-(* So we can define:                                                          *)
-(*             cexec_event_structure == subtype of fin_exec_event_structure   *)
-(*                where reads and corresponding writes are conflict-free and  *)
-(*                thus conflict relation is irreflexive                       *)
+(* ica x y == x is the predecessor of y or y reads from x, ica stands for     *)
+(*            immediate causality relation.                                   *)
+(*      ca == non-strict casuality relation, i.e. the reflexive-transitive    *)
+(*              closure of ica.                                               *)
+(* e1 # e2 == e1 and e2 are conflicting events.                               *)
+(*                                                                            *)
+(* One can prove irreflexivity of the conflict relation under the assumption  *)
+(* that reads are not in conflict with the writes they read from:             *)
+(*   cexec_event_structure == a subtype of finite execution event structures  *)
+(*                            with irreflexive conflict relation              *)
 (******************************************************************************)
 
 Import Order.LTheory.
@@ -56,17 +52,17 @@ Inductive label {Rval Wval : Type} :=
 
 Section PrimeEventStructure.
 
-Context {val : eqType}.
+Context {V : eqType}.
 
 (* ************************************************************************* *)
 (*     Label                                                                 *)
 (* ************************************************************************* *)
 
-Local Notation label := (@label val val).
+Local Notation label := (@label V V).
 
-Implicit Type (l : label).
+Implicit Type l : label.
 
-Definition eq_label l l' := 
+Definition eq_label l l' :=
   match l, l' with
   | Read a x,  Read b y      => [&& a == b & x == y]
   | Write a x, Write b y     => [&& a == b & x == y]
@@ -76,7 +72,7 @@ Definition eq_label l l' :=
   end.
 
 Lemma eqlabelP : Equality.axiom eq_label.
-Proof. 
+Proof.
   case=> [v x [] * /=|v x []* /=|[]|[]]; try constructor=>//;
   by apply: (iffP andP)=> [[/eqP->/eqP->]|[->->]].
 Qed.
@@ -84,17 +80,31 @@ Qed.
 Canonical label_eqMixin := EqMixin eqlabelP.
 Canonical label_eqType := Eval hnf in EqType label label_eqMixin.
 
-Definition is_read  l := if l is (Read _ _) then true else false.
+(* label location *)
+Definition lloc (l : label) :=
+  match l with
+  | Write x _ => Some x
+  | Read  x _ => Some x
+  | _         => None
+  end.
+
+Definition is_read l := if l is (Read _ _) then true else false.
+
+Definition is_write l := if l is Write _ _ then true else false.
 
 Definition is_thdstart l := if l is ThreadStart then true else false.
 
-Definition write_read_from (w r : label) := 
+Definition write_read_from (w r : label) :=
   match w, r with
-  | (Write x a), (Read y b) => (x == y) && (a == b)
-  | _, _                    => false
+  | Write x a, Read y b => (x == y) && (a == b)
+  | _, _ => false
   end.
 
 Notation "w << r" := (write_read_from w r) (at level 0).
+
+Lemma rf_thdend w : w << ThreadEnd = false.
+Proof. by case: w. Qed.
+
 
 (* ************************************************************************* *)
 (*     Exec Event Structure                                                  *)
@@ -103,61 +113,97 @@ Notation "w << r" := (write_read_from w r) (at level 0).
 Structure fin_exec_event_struct {disp} (E : identType disp) := Pack {
   dom        : seq E;
   dom_sorted : sorted (>%O) dom;
-  lab        : rfsfun (fun=> ThreadEnd) dom (fun _ _ => true);
-  ffpred     : rfsfun id dom (>=%O : rel E);
-  ffrf       : rfsfun id dom
-               [rel r w : E | (w <= r) &&
-               (((w == r) && ~~ is_read (lab r)) || ((lab w) << (lab r)))]
+  (* lprf stands for label, predecessor, reads-from *)
+  lprf       : {fsfun for fun e => (ThreadEnd, e, e)};
+  lab e      := (lprf e).1.1;  (* lab is 1st projection *)
+  fpred e    := (lprf e).1.2;  (* fpred is 2nd projection *)
+  frf e      := (lprf e).2;    (* frf is 3d projection *)
+  _          : {subset (finsupp lprf) <= dom};
+  _          : forall e : E, fpred e <= e;
+  _          : forall r : E, let w := frf r in
+                 (w <= r) &&
+                 (((w == r) && ~~ is_read (lab r)) || ((lab w) << (lab r)));
 }.
 
 Section ExecEventStructure.
 
-Context {disp} {E : identType disp} (es : (fin_exec_event_struct E)).
+Context {disp} {E : identType disp} (es : fin_exec_event_struct E).
 
 Notation domain := (dom es).
-Notation lab     := (lab es).
-Notation ffpred   := (ffpred es).
-Notation ffrf     := (ffrf es).
+Notation lprf := (lprf es).
+Notation lab := (lab es).
+Notation fpred := (fpred es).
+Notation frf := (frf es).
 
-(* ************************************************************************* *)
-(*     Event Types                                                           *)
-(* ************************************************************************* *)
+Lemma labE e : lab e = (lprf e).1.1.
+Proof. by []. Qed.
+
+Lemma fpredE e : fpred e = (lprf e).1.2.
+Proof. by []. Qed.
+
+Lemma frfE e : frf e = (lprf e).2.
+Proof. by []. Qed.
+
+
+Lemma lprf_dom : {subset (finsupp lprf) <= domain}.
+Proof. by case: es. Qed.
+
+(***** Labels and Freshness *****)
+Section LabelsFresh.
+
+Notation fresh_id := (fresh_seq domain).
+
+Lemma lab_fresh : lab fresh_id = ThreadEnd.
+Proof.
+  rewrite /lab fsfun_dflt //; apply/negP=> /lprf_dom; apply/negP.
+  by rewrite fresh_seq_notin ?dom_sorted.
+Qed.
+
+End LabelsFresh.
 
 (* ************************************************************************* *)
 (*     Predecessor                                                           *)
 (* ************************************************************************* *)
 
-Definition fpred : E -> E := ffpred.
+Lemma fpred_le e : fpred e <= e.
+Proof. by case: es. Qed.
 
-Lemma fpred_le e: fpred e <= e.
-Proof. 
-  case I: (e \in domain); first exact (axiom_rfsfun ffpred I).
-  by rewrite /fpred (memNdom _ (negbT I)).
+Lemma fpred_domain e :
+  e \notin domain -> fpred e = e.
+Proof.
+  move=> ndom; rewrite /fpred fsfun_dflt //; move: ndom.
+  by apply/contra/lprf_dom.
 Qed.
 
 (* ************************************************************************* *)
 (*     Reads-From                                                            *)
 (* ************************************************************************* *)
 
-Definition frf : E -> E := ffrf.
+Lemma frf_cond r : let w := frf r in
+  (w <= r) &&
+  (((w == r) && ~~ is_read (lab r)) || ((lab w) << (lab r))).
+Proof. by case: es. Qed.
 
 Lemma frf_le r : frf r <= r.
-Proof.
-  case I: (r \in domain); first by case/andP: (axiom_rfsfun ffrf I).
-  by rewrite /frf (memNdom _ (negbT I)).
-Qed.
+Proof. by case/andP: (frf_cond r). Qed.
 
-Lemma frf_domain e: (e \in domain) = false ->
-  frf e = e.
-Proof. by move/negbT/(memNdom ffrf). Qed.
+Lemma frf_lt {e1 e2} : e1 < e2 -> frf e1 < e2.
+Proof. by apply/le_lt_trans/frf_le. Qed.
+
+Lemma frf_domain e :
+  e \notin domain -> frf e = e.
+Proof.
+  move=> ndom; rewrite /frf fsfun_dflt //; move: ndom.
+  by apply/contra/lprf_dom.
+Qed.
 
 Definition fica e := [:: frf e; fpred e].
 
-Lemma fica_domain e: (e \in domain) = false ->
-  fica e = [:: e; e].
-Proof. by move/negbT/[dup]/(memNdom ffpred)=> {4}<- /(memNdom ffrf) {2}<-. Qed.
+Lemma fica_domain e :
+  e \notin domain -> fica e = [:: e; e].
+Proof. by move=> nI; rewrite /fica frf_domain // fpred_domain. Qed.
 
-Lemma fica_le e1 e2: e1 \in (fica e2) -> e1 <= e2.
+Lemma fica_le e1 e2: e1 \in fica e2 -> e1 <= e2.
 Proof. rewrite ?inE=> /orP[]/eqP->; by rewrite (frf_le, fpred_le). Qed.
 
 (* ************************************************************************* *)
@@ -165,75 +211,100 @@ Proof. rewrite ?inE=> /orP[]/eqP->; by rewrite (frf_le, fpred_le). Qed.
 (* ************************************************************************* *)
 
 (* Immediate causality relation *)
-Definition ica e1 e2: bool := e1 \in fica e2.
-
-Arguments ica /.
+Definition ica e1 e2 : bool := e1 \in fica e2.
 
 Lemma ica_le e1 e2 : ica e1 e2 -> e1 <= e2.
-Proof. by move/fica_le. Qed.
-
-Arguments clos_rtn1_rt {_ _ _ _}.
-Arguments clos_rt_rt1n {_ _ _ _}.
-Arguments clos_rt_rtn1 {_ _ _ _}.
-Arguments clos_rt1n_rt {_ _ _ _}.
+Proof. exact: fica_le. Qed.
 
 (* Causality relation *)
 Definition ca : rel E := rt_closure fica fica_le.
 
-Lemma closureP {e1 e2} :
-  reflect (clos_refl_trans_n1 _ ica e1 e2) (ca e1 e2).
-Proof. exact/(equivP (rt_closure_n1P _ _ _ _)). Qed.
+Lemma closureP e1 e2 :
+  reflect (clos_refl_trans_n1 ica e1 e2) (ca e1 e2).
+Proof. exact/(equivP rt_closure_n1P). Qed.
 
-Lemma fica_ca e1 e2: e1 \in fica e2 -> ca e1 e2.
-Proof. 
-  move=> H. apply/closureP/(Relation_Operators.rtn1_trans); first exact: H.
-  exact: rtn1_refl.
-Qed.
+Lemma ica_ca e1 e2 : ica e1 e2 -> ca e1 e2.
+Proof. exact: rt_closure_subrel. Qed.
 
-Lemma ca_refl: reflexive ca.
+Lemma ica_fpred {e}: ica (fpred e) e.
+Proof. by rewrite /ica !inE eqxx. Qed.
+
+Lemma ica_notdom e1 e2:
+  e2 \notin domain ->
+  ica e1 e2 ->
+  e1 == e2.
+Proof. by move=> Ndom2; rewrite /ica fica_domain // !inE orbb. Qed.
+
+Lemma ca_refl {e} : ca e e.
 Proof. exact: rt_closure_refl. Qed.
 
-Lemma ca_trans: transitive ca. 
-Proof. move=>???. exact: rt_closure_trans. Qed.
+Hint Resolve ca_refl : core.
+
+Lemma ca_trans: transitive ca.
+Proof. exact: rt_closure_trans. Qed.
 
 Arguments ca_trans {_ _ _}.
 
-Lemma ca_le e1 e2 : ca e1 e2 -> e1 <= e2.
-Proof. 
-  move/closureP.
-  by elim=> [] // ??/ica_le L ? /le_trans /(_ L).
-Qed.
-
-Lemma ca_decr e1 e2 : e1 != e2 -> ca e1 e2 ->
-  exists e3, [&& ca e1 e3, ica e3 e2 & e3 < e2]. 
-Proof.
-  move/[swap]/closureP/clos_rtn1_rt/clos_rt_rt1n; elim=> [?/eqP//|].
-  move=> x y z I /clos_rt1n_rt/clos_rt_rtn1/closureP L.
-  case N: (y != z). 
-  - case/(_ erefl)=> e /and3P[C *]; exists e; apply/and3P; split=> //.
-    exact/(ca_trans _ C)/fica_ca.
-  move/eqP: N I L=> -> I ?? N; exists x.
-  by rewrite ca_refl I /= lt_def eq_sym N /= ica_le.
-Qed.
-
 Lemma ca_anti: antisymmetric ca.
+Proof. exact: rt_closure_antisym. Qed.
+
+Lemma ca_le e1 e2 : ca e1 e2 -> e1 <= e2.
+Proof. exact: rt_closure_le. Qed.
+
+Lemma ca_step_last e1 e3 :
+  e1 != e3 ->
+  ca e1 e3 ->
+  exists e2, [&& ca e1 e2, ica e2 e3 & e2 < e3].
 Proof.
-  move=> x y /andP[/ca_le Eq /ca_le ?]. 
-  by rewrite (@le_anti _ _ x y) // Eq.
+  move/[swap]/closureP; elim=> [/eqP//|] e2 {}e3.
+  case: (eqVneq e2 e3)=> [-> _ //| neq23 I23 /closureP C12 _ neq13].
+  by exists e2; rewrite C12 I23 lt_neqAle neq23 ica_le.
 Qed.
 
-Lemma ca_fpred {e}: ca (fpred e) e.
+Lemma ca_fpredl {e} : ca (fpred e) e.
+Proof. exact/ica_ca/ica_fpred. Qed.
+
+Lemma ca_fpredr e1 e2 : ca e1 (fpred e2) -> ca e1 e2.
+Proof. by move/ca_trans/(_ ca_fpredl). Qed.
+
+Lemma ca_notdom e1 e2:
+  ca e1 e2 -> e2 \notin domain ->
+  e1 == e2.
 Proof.
-  case Eq: (fpred e != e); last (move/eqP: Eq->; by rewrite ca_refl).
-  by apply/fica_ca; rewrite ?inE eq_refl.
+  move/closureP; elim=> // {}e2 e3 + _ + N3.
+  by move=> /(ica_notdom N3) /eqP-> /(_ N3).
 Qed.
 
-Lemma ca_codom e1 e2: ca e1 e2 -> (e2 \in domain) = false ->
-  (e1 == e2).
-Proof. 
-  move/closureP; elim=> //?? I ? Y Z; move: I Y.
-  by rewrite /ica fica_domain // ?inE orbb=> /eqP-> /(_ Z).
+Definition seqpred_ca := up_set fica fica_le.
+
+Lemma seqpred_ca_in e1 e2: e1 \in seqpred_ca e2 = ca e1 e2.
+Proof. by []. Qed.
+
+(***** Causality and Freshness *****)
+Section CausalityFresh.
+
+Notation fresh_id := (fresh_seq domain).
+
+Lemma ica_fresh e: ica fresh_id e -> e = fresh_id.
+Proof.
+  move/[dup]/ica_ca/ca_notdom/[swap]/fica_le.
+  rewrite /ica ?inE.
+  case I: (e \in domain); last by move=> ?/(_ erefl)/eqP->.
+  by move/lt_geF: (fresh_seq_lt (dom_sorted es) I)=>->.
 Qed.
+
+Lemma ca_fresh e: ca fresh_id e -> e = fresh_id.
+Proof. by move/closureP; elim=> // ?? /[swap] ? /[swap]-> /ica_fresh. Qed.
+
+Lemma ca_fresh2 e1 e2 :
+  ca e1 e2 -> e1 = fresh_id -> e2 = fresh_id.
+Proof. by move/[swap]->; apply: ca_fresh. Qed.
+
+Lemma ca_fresh_contra e1 e2 :
+  e2 != fresh_id -> ca e1 e2 -> e1 != fresh_id.
+Proof. by move=> nfr2 /ca_fresh2/contra_neq->. Qed.
+
+End CausalityFresh.
 
 (*Lemma ca_dom e1 e2: ca e1 e2 -> (e1 \in domain) = false ->
   e1 = e2.
@@ -265,125 +336,120 @@ Notation "x <c= y" := (@Order.le ev_display _ x y) (at level 0).*)
 (* ************************************************************************* *)
 
 (* Immediate conflict relation *)
-Definition icf (e1 e2 : E) :=
-  [&& (e1 != e2),
+Definition icf (e1 e2 : E) : bool :=
+  [&& e1 != e2,
       fpred e1 == fpred e2,
       fpred e1 < e1,
       fpred e2 < e2,
       ~~ is_thdstart (lab e1) &
       ~~ is_thdstart (lab e2)].
 
-Lemma icf_symm e1 e2: icf e1 e2 -> icf e2 e1.
-Proof. 
-  case/and5P=>*. 
-  by apply/and5P; split=> //; rewrite 1?eq_sym // andbC.
+Lemma icfxx x : icf x x = false.
+Proof. by apply/and6P; case; rewrite eq_refl. Qed.
+
+Hint Resolve icfxx : core.
+
+Lemma icf_sym : symmetric icf.
+Proof.
+  by move=> e1 e2; apply/and6P/and6P; case=>*; split=> //; rewrite 1?eq_sym.
 Qed.
 
-Definition seqpred_ca := up_set fica fica_le .
-
-Lemma seqpred_ca_in e1 e2: e1 \in seqpred_ca e2 = ca e1 e2.
-Proof. by []. Qed.
-
 (* Conflict relation *)
-Definition cf e1 e2 :=
-  has (fun p=> icf p.1 p.2)
-  (allpairs pair (seqpred_ca e1) (seqpred_ca e2)).
+Definition cf e1 e2 : bool :=
+  has id [seq icf x y | x <- seqpred_ca e1, y <- seqpred_ca e2].
 
 Notation "a # b" := (cf a b) (at level 10).
 
-Lemma cfP {e1 e2}:
-  reflect (exists e1' e2', [&& ca e1' e1, ca e2' e2 & icf e1' e2']) (e1 # e2).
+Lemma cfP {e1 e2} :
+  reflect (exists e1' e2', (ca e1' e1 * ca e2' e2 * icf e1' e2')%type) (e1 # e2).
 Proof.
-  apply/(iffP hasP)=> [[? /allpairsPdep[x[y[]]]]|[x [y /and3P[]]]].
-  - rewrite 2!seqpred_ca_in=> ?? -> /= ?.
-    exists x, y; exact /and3P.
-  rewrite -2!seqpred_ca_in=> *.
-  exists (x, y)=> //; exact /allpairs_f. 
+  apply/(iffP hasP)=> [[? /allpairsPdep[x[y[]]]]|[x [y [[]]]]].
+  - by rewrite 2!seqpred_ca_in=> ?? -> /= ?; exists x, y.
+    by exists (icf x y)=> //; rewrite allpairs_f.
 Qed.
 
-Lemma cf_symm: symmetric cf.
+Lemma cf_sym: symmetric cf.
 Proof.
-  move=> *. apply /(sameP idP) /(iffP idP) => /cfP[x [y /and3P[*]]].
-  all: apply/cfP; exists y, x.
-  all: by apply/and3P; split=> //; apply/icf_symm.
+  apply: symmetric_from_pre=> e1 e2 /cfP [e1' [e2'] Cf].
+  by apply/cfP; exists e2', e1'; rewrite icf_sym !Cf.
 Qed.
 
-Lemma consist_cf {e1 e2 e3 e4}: e1 # e2 -> ca e1 e3 -> ca e2 e4 -> e3 # e4.
+Lemma cf_consist2 e1 e2 e3 e4 :
+  e1 # e2 -> ca e1 e3 -> ca e2 e4 -> e3 # e4.
 Proof.
-  move=> /cfP[x [y/and3P[C C' ???]]].
-  apply/cfP; exists x, y.
-  apply/and3P; split=>//; by rewrite ((ca_trans C), (ca_trans C')).
+  move=> /cfP[e1' [e2'] [[/ca_trans C1] /ca_trans C2 *]].
+  by apply/cfP; exists e1', e2'; rewrite C1 // C2.
 Qed.
 
-Notation cf_step e1 e2 := 
+Lemma cf_consistl e1 e2 e3 :
+  ca e1 e3 -> e1 # e2 -> e2 # e3.
+Proof. by move=> C13 /cf_consist2 /(_ C13); rewrite cf_sym=>->. Qed.
+
+Lemma cf_consistr e1 e2 e3 :
+  ca e2 e3 -> e1 # e2 -> e1 # e3.
+Proof. by rewrite cf_sym; apply: cf_consistl. Qed.
+
+Lemma icf_cf e1 e2: icf e1 e2 -> e1 # e2.
+Proof. by move=> I; apply/cfP; exists e1, e2; rewrite !ca_refl I. Qed.
+
+Notation cf_step e1 e2 :=
   [|| icf e1 e2,
       has (cf e1) (fica e2) |
       has (cf e2) (fica e1)].
 
-Lemma icf_cf e1 e2: icf e1 e2 -> e1 # e2.
-Proof.
-  move=> I; apply/cfP.
-  exists e1, e2; by rewrite ?ca_refl I.
-Qed.
-
 Lemma cf_step_cf e1 e2: cf_step e1 e2 -> e1 # e2.
 Proof.
-  case/or3P=> [/icf_cf||]// /hasP[? /fica_ca /[swap] /consist_cf /[apply]];
-  last rewrite cf_symm; apply; by rewrite ca_refl.
+  case/or3P=> [/icf_cf //||] /hasP[e /ica_ca]; first by apply: cf_consistr.
+  by move=> /cf_consistr /[apply]; rewrite cf_sym.
 Qed.
 
 Lemma cfE e1 e2: e1 # e2 = cf_step e1 e2.
 Proof.
-  apply /(sameP idP)/(iffP idP)=> [/cf_step_cf | /cfP] //.
-  case=> ? [? /and3P[/closureP]].
-  elim=> [/closureP | ?? /[swap] ?].
-  - elim=> [-> |] // ?? /[swap] _.
-    rewrite /ica ?inE=> /orP[]/eqP-> /[apply] /cf_step_cf /= -> //=;
-    by rewrite orbT.
-  rewrite /ica ?inE=> /orP[]/eqP-> /[apply]/[apply] /cf_step_cf /=;
-  by rewrite cf_symm=> /= ->.
+  apply/idP/idP; last by apply: cf_step_cf.
+  case/cfP=> e1' [e2' [[/closureP]]].
+  elim=> [/closureP | ?? /[swap] _ + /[apply] + /[apply] + /cf_step_cf].
+  - elim=> [-> //| ?? + _ /[apply] + /cf_step_cf].
+    by rewrite /ica !inE=> /pred2P[]-> /= ->; rewrite orbT.
+  by rewrite cf_sym /ica ?inE=> /pred2P[]-> /= ->.
 Qed.
 
 (* ************************************************************************* *)
 (*     Reads-From Consistency                                                *)
 (* ************************************************************************* *)
 
-Definition consistency :=  all (fun e => ~~ e # (frf e)) domain.
+Definition dom_consistency :=  all (fun e => ~~ (e # (frf e))) domain.
 
-Hypothesis consist : consistency.
+Hypothesis Consistent : dom_consistency.
 
-Lemma rff_consist e : ~ e # (frf e).
+Lemma rff_consist e : e # (frf e) = false.
 Proof.
-  case D: (e \in domain).
-  - apply/negP; by move/allP/(_ _ D): consist.
-  rewrite frf_domain // => /cfP[? [? /and3P[/ca_codom/(_ D) /eqP ->]]].
-  by move/ca_codom/(_ D)/eqP-> => /andP[/negP].
+  apply/negbTE/negP; case: (boolP (e \in domain)) => [D|nD].
+  - by move/allP/(_ _ D)/negP: Consistent.
+  rewrite frf_domain // => /cfP[e1 [e2 [[]]]]; do 2 move/ca_notdom/(_ nD)/eqP->.
+  by rewrite icfxx.
 Qed.
 
 Lemma cf_irrelf : irreflexive cf.
 Proof.
-  move=> m; apply/negbTE/negP.
-  elim/(@wfb_ind disp E): m=> m IHn.
-  suff C: ~ m # (fpred m).
-  - by rewrite cfE /icf=> /or3P[/andP[/eqP]||] //= /or3P[]// /rff_consist.
-  move=> /cfP[x [y /and3P[]]]; case Eq: (x == m).
-  - move/eqP :Eq =>-> ? /ca_le L /and5P[?/eqP<- ?] /(le_lt_trans L).
-    by rewrite ltxx.
-  move/negbT/ca_decr: Eq => /[apply] [[z /and3P[/[swap]]]].
-  rewrite /ica=> /or3P[]// /eqP-> C1 ?.
-  - move/ca_trans /(_ ca_fpred)=> ? /icf_cf; rewrite cf_symm=> C. 
-    exact/(@rff_consist m)/(consist_cf C).
-  move=> C2 /icf_cf /consist_cf/(_ C1 C2); exact/IHn.
+  move=> m; apply/negbTE/negP; elim/(@wfb_ind disp E): m=> m IHm.
+  suff C: ~ m # (fpred m) by rewrite cfE icfxx orbb /= rff_consist /= orbF.
+  move=> /cfP[x [y [[]]]]; case: (eqVneq x m)=> [-> _|].
+  - by move=> /ca_le L /and6P[_ /eqP<- _ /(le_lt_trans L)]; rewrite ltxx.
+  move/ca_step_last=> /[apply] [[z /and3P[/[swap]]]].
+  rewrite /ica !inE=> /pred2P[]-> Cx ?.
+  - move=> /ca_fpredr Cy /icf_cf/cf_consist2/(_ Cx Cy).
+    by rewrite cf_sym rff_consist.
+  by move=> Cy /icf_cf/cf_consist2/(_ Cx Cy); exact/IHm.
 Qed.
 
 End ExecEventStructure.
 
 Section Consistency.
 
-Context {disp}{E : identType disp}.
+Context {disp : unit} {E : identType disp}.
 Implicit Type es : (@fin_exec_event_struct disp E).
 
-Inductive cexec_event_struct := Consist es of (consistency es).
+Inductive cexec_event_struct := Consist es of (dom_consistency es).
 
 Arguments Consist {_}.
 
@@ -401,6 +467,4 @@ End PrimeEventStructure.
 
 (*Notation "x <c= y" := (@Order.le ev_display _ x y) (at level 10).*)
 Notation "a # b" := (cf _ a b) (at level 10).
-Notation "w << r" := (write_read_from w r) (at level 0). 
-
-Arguments cfP {val disp E es e1 e2}.
+Notation "w << r" := (write_read_from w r) (at level 0).
